refactored list_utils in pcc4irm, late npc reduction

coq/pcc/list_utils.v
@@ -1,345 +1,215 @@
-
-Set Implicit Arguments.
-
 Require Export List.
 Require Import Arith.
 Require Import Omega.
+Require Import ssreflect.
 
-Section list_utils.
+Set Implicit Arguments.
 
-  Variable A : Set.
-  
-  Lemma app_cons_has_head : forall (a : A) l l', exists a', exists l'', l ++ a :: l' = a' :: l''.
-  Proof.
-    intros.
-    destruct l.
-    exists a; exists l'.
-    reflexivity.
-    exists a0; exists (l ++ a :: l').
-    reflexivity.
-  Qed.
-  
-  
-  Lemma nil_or_app : forall l, l = nil \/ exists l', exists a: A, l = l' ++ a :: nil.
-    intros.
-    induction l.
-    left; reflexivity.
-    right.
-    elim IHl; intros.
-    exists nil.
-    exists a.
-    subst; reflexivity.
-    elim H; intros.
-    elim H0; intros.
-    subst.
-    exists (a::x).
-    exists x0.
-    reflexivity.
-  Qed.
-  
-  
-  Lemma in_but_not_last : forall l (a b: A), In a (l ++ b :: nil) -> a = b \/ In a l.
-    intros.
-    apply In_rev in H.
-    rewrite distr_rev in H.
-    simpl in H.
-    elim H; intros.
-    left.
-    auto.
-    right.
-    apply In_rev in H0.
-    assumption.
-  Qed.
-  
+Section ListUtils.
 
-  Lemma list_rearrange : forall l l' (a:A), l ++ a :: l' = (l ++ a :: nil) ++ l'.
-    intros.
-    induction l.
-    induction l'; simpl; auto.
-    rewrite app_ass.
-    trivial.
-  Qed.
-  
-  
-  Lemma list_rearrange2 : forall l (a b: A), l ++ a :: b :: nil = (l ++ a :: nil) ++ b :: nil.
-    intros.
-    rewrite app_ass.
-    auto with datatypes.
-  Qed.
-  
+Variable A : Set.
 
-  Lemma list_rearrange3 : forall l l' (a : A), (a :: l) ++ l' = a :: l ++ l'.
-    reflexivity.
-  Qed.
+Lemma app_cons_has_head : forall (a : A) l l', exists a', exists l'', l ++ a :: l' = a' :: l''.
+Proof. 
+move => a; case => [l'|a' l l']; first by exists a; exists l'. 
+by exists a'; exists (l ++ a :: l'). 
+Qed.
 
-  
-  Lemma list_neq_length : forall l l': list A, length l <> length l' -> l <> l'.
-    intros.
-    contradict H.
-    subst.
-    reflexivity.
-  Qed.
+Lemma nil_or_app : forall l, l = nil \/ exists l', exists a: A, l = l' ++ a :: nil.
+Proof.
+elim => [|a l IHl]; first by left.
+right; elim: IHl => H; first by exists nil; exists a; rewrite H.
+by move: H => [l' [a' H]]; exists (a :: l'); exists a'; rewrite H.
+Qed.
 
-  
-  Inductive prefix : list A -> list A -> Prop :=
-  | prefix_nil : forall l, prefix nil l
-  | prefix_next : forall (a: A) l l', prefix l l' -> prefix (a :: l) (a :: l').
-  
+Lemma in_but_not_last : forall l (a b: A), In a (l ++ b :: nil) -> a = b \/ In a l.
+Proof.
+move => l a b H.
+apply In_rev in H.
+rewrite distr_rev /= in H.
+by elim: H => H; [ left | right; apply In_rev in H ].
+Qed.
 
-  Lemma prefix_firstn : forall n (l : list A), n <= length l -> prefix (firstn n l) l.
-    induction n; intros.
-    apply prefix_nil.
-    destruct l.
-    inversion H.
-    simpl.
-    apply prefix_next.
-    apply IHn.
-    apply le_S_n; assumption.
-  Qed.
-  
-  
-  Inductive proper_prefix : list A -> list A -> Prop :=
-  | proper_prefix_nil : forall (l: list A) a, proper_prefix nil (a :: l)
-  | proper_prefix_next : forall a l l', proper_prefix l l' -> proper_prefix (a :: l) (a :: l').
-  
-  
-  Lemma proper_prefix_app : forall (l l' l'': list A), proper_prefix l l' -> proper_prefix (l''++l) (l''++l').
-    intros.
-    induction l''.
-    assumption.
-    repeat rewrite <- app_comm_cons.
-    apply proper_prefix_next.
-    assumption.
-  Qed.
-  
-  
-  Lemma proper_prefix_last : forall l (a: A), proper_prefix l (l ++ a :: nil).
-    intros.
-    induction l.
-    apply proper_prefix_nil.
-    rewrite <- app_comm_cons.
-    apply proper_prefix_next.
-    assumption.
-  Qed.
-  
-  
-  Lemma proper_prefix_split : forall (l l': list A), proper_prefix l' l -> exists x, exists l'', l = l' ++ (x :: l'').
-    induction l; intros.
-    inversion H.
-    destruct l'.
-    exists a.
-    exists l.
-    auto.
-    inversion H; subst.
-    apply IHl in H1.
-    inversion H1.
-    inversion H0.
-    subst.
-    exists x.
-    exists x0.
-    auto.
-  Qed.
-  
+Lemma list_rearrange : forall l l' (a:A), l ++ a :: l' = (l ++ a :: nil) ++ l'.
+Proof. by elim => [|a l IH l' a']; [ case | rewrite app_ass ]. Qed.
 
-  Lemma proper_prefix_shorter : forall (l' l: list A), proper_prefix l' l -> length l' < length l.
-    intros.
-    apply proper_prefix_split in H.
-    inversion H; subst.
-    inversion H0; subst.
-    rewrite app_length.
-    simpl.
-    omega.
-  Qed.
-  
-  
-  Theorem proper_prefix_well_founded : well_founded (@proper_prefix).
-    apply well_founded_lt_compat with (f := @length A).
-    apply proper_prefix_shorter.
-  Qed.
-  
-  
-  Theorem strong_list_ind (P: list A -> Prop) :
-    (forall l, (forall l', proper_prefix l' l -> P l') -> P l) -> forall l, P l.
-    intros P H.
-    apply well_founded_ind with (R := @proper_prefix).
-    apply proper_prefix_well_founded.
-    intros.
-    apply H.
-    intros.
-    apply H0.
-    assumption.
-  Qed.
-  
-  
-  Lemma in_list_in_prefix : forall l l' (a: A), proper_prefix l' l -> In a l' -> In a l.
-    intros.
-    apply proper_prefix_split in H.
-    elim H; intros.
-    elim H1; intros.
-    rewrite H2.
-    apply in_or_app.
-    left.
-    assumption.
-  Qed.
-  
-  
-  Lemma nil_or_last : forall l, l = nil \/ exists l', exists a : A, l = l' ++ a :: nil.
-    intros.
-    destruct l using rev_ind.
-    left; reflexivity.
-    right.
-    exists l.
-    exists x.
-    reflexivity.
-  Qed.
-  
-  
-  Inductive suffix : list A -> list A -> Prop :=
-  | suffix_here : forall (l: list A), suffix l l
-  | suffix_next : forall a suff l, suffix suff l -> suffix suff (a::l).
-  
-  
-  Lemma suffix_split :
-    forall l suff: list A, suffix suff l -> exists pref, l = pref ++ suff.
-  Proof.
-    intros l.
-    induction l; intros.
-    inversion H; subst.
-    exists nil.
-    reflexivity.
-    inversion H; subst.
-    exists nil.
-    reflexivity.
-    apply IHl in H2.
-    elim H2; intros.
-    subst.
-    exists (a::x).
-    reflexivity.
-  Qed.
-  
-  
-  Lemma suffix_app :
-    forall l l' l'': list A, suffix l l' -> suffix l (l'' ++ l').
-  Proof.
-    intros.
-    induction l''.
-    assumption.
-    simpl.
-    apply suffix_next.
-    assumption.
-  Qed.
-  
-  
-  Lemma suffix_transitive :
-    forall c bc abc: list A, suffix bc abc -> suffix c bc -> suffix c abc.
-  Proof.
-    intros.
-    apply suffix_split in H.
-    apply suffix_split in H0.
-    elim H; intros.
-    elim H0; intros.
-    subst.
-    apply suffix_app.
-    apply suffix_app.
-    apply suffix_here.
-  Qed.
-  
-  
-  Inductive last : list A -> A -> Prop :=
-  | last_base : forall a, last (a :: nil) a
-  | last_cons : forall l a b, last l a -> last (b::l) a.
+Lemma list_rearrange2 : forall l (a b: A), l ++ a :: b :: nil = (l ++ a :: nil) ++ b :: nil.
+Proof. by move => l a b; rewrite app_ass. Qed.
 
+Lemma list_rearrange3 : forall l l' (a : A), (a :: l) ++ l' = a :: l ++ l'.
+Proof. by []. Qed.
 
-  Lemma last_exists : forall l (c : A), exists c', last (c :: l) c'.
-  Proof.
-    intros.
-    induction l.
-    exists c.
-    apply last_base.
-    elim IHl; intros.
-    inversion H; subst.
-    exists a.
-    apply last_cons.
-    apply last_base.
-    exists x.
-    apply last_cons.
-    apply last_cons.
-    assumption.
-  Qed.
+Lemma list_neq_length : forall l l': list A, length l <> length l' -> l <> l'.
+Proof. by move => l l' H; contradict H; rewrite H. Qed.
 
+Inductive prefix : list A -> list A -> Prop :=
+| prefix_nil : forall l, prefix nil l
+| prefix_next : forall (a: A) l l', prefix l l' -> prefix (a :: l) (a :: l').
 
-  Lemma single_last : forall l (a b: A), last l a -> last l b -> a = b.
-    intros.
-    induction l.
-    inversion H.
-    inversion H; subst.
-    inversion H0; subst.
-    reflexivity.
-    inversion H4.
-    apply IHl.
-    assumption.
-    inversion H0; subst.
-    inversion H4.
-    assumption.
-  Qed.
+Lemma prefix_firstn : forall n (l : list A), n <= length l -> prefix (firstn n l) l.
+Proof.
+elim => [l H|n IHn]; first by apply prefix_nil.
+case => [|a l] H; first by inversion H.
+by apply prefix_next; apply IHn; apply le_S_n.
+Qed.
 
-  
-  Lemma last_app : forall l l' (a: A), last l' a -> last (l++l') a.
-    intros.
-    induction l.
-    simpl.
-    assumption.
-    simpl.
-    apply last_cons.
-    assumption.
-  Qed.
-  
-  
-  Lemma app_last : forall l (a: A), last (l ++ a :: nil) a.
-  Proof.
-    intros.
-    induction l.
-    apply last_base.
-    rewrite list_rearrange3.
-    apply last_cons.
-    assumption.
-  Qed.
+Inductive proper_prefix : list A -> list A -> Prop :=
+| proper_prefix_nil : forall (l: list A) a, proper_prefix nil (a :: l)
+| proper_prefix_next : forall a l l', proper_prefix l l' -> proper_prefix (a :: l) (a :: l').
 
-  
-  Lemma last_app_prefix :
-    forall (l l': list A) a, last l a -> exists l', l = l' ++ a::nil.
-  Proof.
-    intros l l'.
-    induction l; intros.
-    inversion H.
-    
-    inversion H; subst.
-    exists nil.
-    auto with datatypes.
-    
-    apply IHl in H3.
-    elim H3; intros.
-    rewrite H0.
-    exists (a::x).
-    auto with datatypes.
-  Qed.
-  
-  
-  Lemma last_app_cons :
-    forall l (a b: A), last (l ++ a::nil) b -> a = b.
-  Proof.
-    intros.
-    apply last_app_prefix in H.
-    elim H; intros.
-    apply app_inj_tail in H0.
-    elim H0; intros; assumption.
-    auto.
-  Qed.
-  
-  
-  Lemma list_same_head :
-    forall l (a b: A), head (l ++ a :: nil) = head (l ++ a :: b :: nil).
-    induction l; intros; reflexivity.
-  Qed.
+Lemma proper_prefix_app : forall (l l' l'': list A), 
+  proper_prefix l l' -> proper_prefix (l'' ++ l) (l'' ++ l').
+Proof.
+move => l l'.
+elim => [|a l'' IH H]; first by [].
+rewrite -2!app_comm_cons.
+by apply proper_prefix_next; apply IH.
+Qed.
 
-End list_utils.
+Lemma proper_prefix_last : forall l (a: A), proper_prefix l (l ++ a :: nil).
+Proof.
+elim => [|a l IH a']; first by apply proper_prefix_nil.
+by rewrite -app_comm_cons; apply proper_prefix_next.
+Qed.
+
+Lemma proper_prefix_split : forall (l l': list A), 
+  proper_prefix l' l -> exists x, exists l'', l = l' ++ (x :: l'').
+Proof.
+elim => [l' H|a l IH]; first by inversion H.
+case => [|a' l'] H; first by exists a; exists l.
+have ->: a = a' by inversion H.
+have H0: proper_prefix l' l by inversion H.
+apply IH in H0.
+move: H0 => [x [l'' H0]].
+by exists x; exists l''; rewrite H0.
+Qed.
+
+Lemma proper_prefix_shorter : forall (l' l: list A), proper_prefix l' l -> length l' < length l.
+Proof.
+move => l' l H.
+apply proper_prefix_split in H.
+move: H => [a' [l'' H]].
+rewrite H app_length /=.
+by omega.
+Qed.
+
+Theorem proper_prefix_well_founded : well_founded (@proper_prefix).
+Proof. 
+apply well_founded_lt_compat with (f := @length A). 
+by apply proper_prefix_shorter. 
+Qed.
+
+Theorem strong_list_ind (P: list A -> Prop) :
+  (forall l, (forall l', proper_prefix l' l -> P l') -> P l) -> forall l, P l.
+Proof.
+move => P H.
+apply well_founded_ind with (R := @proper_prefix).
+apply proper_prefix_well_founded.
+move => x H0.
+apply H => l' H1.
+by apply H0.
+Qed.
+
+Lemma in_list_in_prefix : forall l l' (a: A), proper_prefix l' l -> In a l' -> In a l.
+Proof.
+move => l l' a H H0.
+apply proper_prefix_split in H.
+move: H => [a' [l'' H]].
+rewrite H.
+by apply in_or_app; left.
+Qed.
+
+Lemma nil_or_last : forall l, l = nil \/ exists l', exists a : A, l = l' ++ a :: nil.
+Proof. by elim/rev_ind => [|a l IH]; [ left | right; exists l; exists a ]. Qed.
+
+Inductive suffix : list A -> list A -> Prop :=
+| suffix_here : forall (l: list A), suffix l l
+| suffix_next : forall a suffx l, suffix suffx l -> suffix suffx (a::l).
+
+Lemma suffix_split : forall l suffx: list A, 
+  suffix suffx l -> exists pref, l = pref ++ suffx.
+Proof.
+elim => [|a l IH] suffx H; first by inversion H; exists nil.
+inversion H; subst; first by exists nil.
+apply IH in H2.
+move: H2 => [l' H2].
+by exists (a :: l'); rewrite H2.
+Qed.
+
+Lemma suffix_app : forall l l' l'': list A, 
+  suffix l l' -> suffix l (l'' ++ l').
+Proof.
+move => l l'.
+elim => [|a l'' IH H]; first by [].
+rewrite /=; 
+by apply suffix_next; apply IH.
+Qed.
+
+Lemma suffix_transitive : forall c bc abc: list A, 
+  suffix bc abc -> suffix c bc -> suffix c abc.
+Proof.
+move => c bc abc H H0. 
+apply suffix_split in H.
+apply suffix_split in H0.
+move: H => [pref H]; move: H0 => [pref' H0].
+rewrite H H0.
+by do 2!apply suffix_app; apply suffix_here.
+Qed.
+
+Inductive last : list A -> A -> Prop :=
+| last_base : forall a, last (a :: nil) a
+| last_cons : forall l a b, last l a -> last (b::l) a.
+
+Lemma last_exists : forall l (c : A), exists c', last (c :: l) c'.
+Proof.
+elim => [|a l IH] c; first by exists c; apply last_base.
+have H: exists c', last (c :: l) c' by apply IH.
+move: H => [c' H] {IH}.
+inversion H; first by exists a; apply last_cons; apply last_base.
+by exists c'; apply last_cons; apply last_cons.
+Qed.
+
+Lemma single_last : forall l (a b: A), last l a -> last l b -> a = b.
+Proof.
+elim => [|a' l IH] a b H H0; first by inversion H.
+inversion H; subst; first by inversion H0; subst; last by inversion H4.
+apply IH; first by [].
+by inversion H0; subst; first by inversion H4.
+Qed.
+
+Lemma last_app : forall l l' (a: A), last l' a -> last (l++l') a.
+Proof.
+elim => [|a' l IH l' a H]; first by [].
+by apply last_cons; apply IH.
+Qed.
+
+Lemma app_last : forall l (a: A), last (l ++ a :: nil) a.
+Proof.
+elim => [|a' l IH] a; first by apply last_base.
+by rewrite list_rearrange3; apply last_cons.
+Qed.
+
+Lemma last_app_prefix : forall (l : list A) (a : A), 
+  last l a -> exists l', l = l' ++ a::nil.
+Proof.
+elim => [|a' l IH] a H; first by inversion H.
+inversion H; subst; first by exists nil.
+apply IH in H3.
+move: H3 => [l'' H3]; rewrite H3 {H3}.
+by exists (a' :: l'').
+Qed.
+
+Lemma last_app_cons :forall l (a b: A), last (l ++ a::nil) b -> a = b.
+Proof.
+move => l a b H.
+apply last_app_prefix in H.
+move: H => [l' H].
+apply app_inj_tail in H.
+by move: H => [H H0].
+Qed.
+
+Lemma list_same_head : forall l (a b: A), 
+  head (l ++ a :: nil) = head (l ++ a :: b :: nil).
+Proof. by case. Qed.
+
+End ListUtils.
